NBE.lean
@@ -6,3 +6,4 @@ import NBE.SingleSortImp.Beta
 import NBE.SingleSortImp.BetaNormalizing
 import NBE.SingleSortImp.BetaEta
 import NBE.SingleSortImp.BetaEtaNormalizing
+import NBE.SingleSortImp.BetaEtaCons
