NBE/SingleSortImp/BetaEtaCons.lean
@@ -1,0 +1,417 @@
+import NBE.SingleSortImp.Presheaf
+import NBE.SingleSortImp.BetaEta
+namespace SingleSortImp
+namespace BetaEtaCons
+
+
+def forces (P: Context -> Tm -> Ty -> Prop) (Γ: Context) (t: Tm) (T: Ty) :=
+  match T with
+  | .Atom =>
+    {t': Tm // t.eq t' ∧ P Γ t' T}
+  | .imp A B =>
+    forall (s: Tm) Γ',
+      forces P (Γ' ++ Γ) s A ->
+      forces P (Γ' ++ Γ) ((t.up 0 Γ'.length).app s) B
+
+
+def forces_eq {P: Context -> Tm -> Ty -> Prop} {Γ: Context} {t1 t2: Tm} {T: Ty}:
+  t1.eq t2 -> forces P Γ t1 T -> forces P Γ t2 T
+:= by
+  intro E F
+  induction T using Ty.ind generalizing t1 t2 Γ with
+  | Atom =>
+    unfold forces at *
+    obtain ⟨t', E', H⟩ := F
+    exists t'
+    and_intros
+    . apply ECl.trans
+      . apply ECl.symm
+        exact E
+      . exact E'
+    . exact H
+  | imp T1 T2 IH1 IH2 =>
+    simp [forces]
+    intro s Γ' F'
+    apply IH2
+    . apply Tm.eq.app1
+      apply E.up
+    . specialize F s Γ'
+      apply F
+      exact F'
+
+mutual
+
+def quote {Γ t T}: forces Tm.NF Γ t T -> {t': Tm // t.eq t' ∧ Tm.NF Γ t' T} :=
+  match T with
+  | .Atom => by
+    simp [forces]
+    intro N
+    exact N
+  | .imp T1 T2 => by
+    simp [forces]
+    intro F
+    have H: Tm.NE (T1 :: Γ) (Tm.var 0) T1 := by
+      constructor
+      simp
+    specialize F (.var 0) [T1]
+    simp at F
+    specialize F (unquote H)
+    obtain ⟨t', E, N⟩ := quote F
+    exists t'.abs
+    and_intros
+    . apply ECl.rstep Tm.step.eta
+      apply Tm.eq.abs
+      exact E
+    . apply Tm.NF.abs
+      exact N
+
+
+def unquote {Γ t T}: Tm.NE Γ t T -> forces Tm.NF Γ t T :=
+  match T with
+  | .Atom => by
+    simp [forces]
+    intro N
+    exists t
+    and_intros
+    . apply ECl.refl
+    . apply Tm.NF.atom
+      exact N
+  | .imp T1 T2 => by
+    intro N
+    simp [forces]
+    intro s Γ' F
+    obtain ⟨s', E, N'⟩ := quote F
+    apply forces_eq
+    . apply Tm.eq.app2
+      apply ECl.symm
+      exact E
+    . apply unquote
+      apply Tm.NE.app
+      . exact N.weaken_app
+      . exact N'
+end
+
+
+def NE.normalize {Γ t T}:
+  Tm.NE Γ t T -> { t': Tm // t.eq t' ∧ Tm.NF Γ t' T }
+:= by
+  intro N
+  replace N := unquote N
+  replace N := quote N
+  exact N
+
+
+namespace Example
+
+def Γ: Context := [.Atom, .imp .Atom .Atom]
+
+def var0_NE: Tm.NE Γ (.var 0) .Atom := by
+  constructor
+  simp [Γ]
+
+
+def var1_NE: Tm.NE Γ (.var 1) (.imp .Atom .Atom) := by
+  constructor
+  simp [Γ]
+
+def var1' := (NE.normalize var1_NE).property
+end Example
+
+
+inductive Satisfy (Δ: Context): Env -> Context -> Type where
+  | nil: Satisfy Δ [] []
+  | cons {T: Ty} {t: Tm} {Γ ts}:
+    forces Tm.NF Δ t T ->
+    Satisfy Δ ts Γ ->
+    Satisfy Δ (t :: ts) (T :: Γ)
+
+
+theorem Satisfy.length {Δ env Γ}:
+  Satisfy Δ env Γ -> env.length = Γ.length
+:= by
+  intro S
+  induction S with
+  | nil =>
+    simp
+  | cons =>
+    simp_all
+
+
+def forces.weaken {Γ Γ' t T}:
+  forces Tm.NF Γ t T -> forces Tm.NF (Γ' ++ Γ) (t.up 0 Γ'.length) T
+:= by
+  intro F
+  induction T using Ty.ind generalizing Γ' with
+  | Atom =>
+    simp [forces]
+    obtain ⟨t', E, N⟩ := F
+    exists (t'.up 0 Γ'.length)
+    and_intros
+    . apply E.up
+    . apply N.weaken_app
+  | imp A B IH1 IH2 =>
+    simp [forces]
+    intro s Γ'' F'
+    simp [Tm.shift_up_add]
+    rewrite [<-List.append_assoc]
+    rewrite [Nat.add_comm]
+    rewrite [<-List.length_append]
+    apply F
+    simp
+    exact F'
+
+
+def Satisfy.weaken {Δ Δ': Context} {Γ env}:
+  Satisfy Δ env Γ -> Satisfy (Δ' ++ Δ) (env.up 0 Δ'.length) Γ
+  | .nil => .nil
+  | .cons F S => .cons F.weaken S.weaken
+
+
+def Satisfy.weaken_cons {Δ A} {Γ env}:
+  Satisfy Δ env Γ -> Satisfy (A :: Δ) (env.up 0 1) Γ
+:= by
+  intro S
+  replace S := S.weaken (Δ' := [A])
+  simp at S
+  exact S
+
+
+def Satisfy.self {Γ}:
+  Satisfy Γ (Env.vars Γ.length) Γ
+:= match Γ with
+  | [] => .nil
+  | T :: TS => by
+    apply Satisfy.cons
+    . apply unquote
+      apply Tm.NE.var
+      simp
+    . apply Satisfy.weaken_cons
+      apply Satisfy.self
+
+
+theorem Satisfy.some_lt {Γ i T} {Δ env}:
+  Satisfy Δ env Γ ->
+  Γ.lookup i = some T ->
+  i < env.length
+:= by
+  intro S H
+  simp_all [S.length]
+  apply FinMap.lookup_some_lt H
+
+
+/--
+I have to redefine this in order to have the constructive proof.
+-/
+inductive Typing: Context -> Tm -> Ty -> Type where
+  | var {Γ: Context} {x: Nat} {T: Ty}:
+    Γ.lookup x = some T ->
+    Typing Γ (.var x) T
+  | abs {Γ: Context} {M: Tm} {T1 T2: Ty}:
+    Typing (T1 :: Γ) M T2 ->
+    Typing Γ (.abs M) (T1.imp T2)
+  | app {Γ: Context} {M N: Tm} {T1 T2: Ty}:
+    Typing Γ M (T1.imp T2) ->
+    Typing Γ N T1 ->
+    Typing Γ (.app M N) T2
+
+
+def Typing.weaken_lemma {Γ1 Γ2 Γ3: Context} {M: Tm} {T}:
+  Typing (Γ1 ++ Γ2) M T ->
+  Typing (Γ1 ++ (Γ3 ++ Γ2)) (M.up Γ1.length Γ3.length) T
+:= by
+  intro HT
+  induction M using Tm.ind generalizing Γ1 Γ2 Γ3 T with
+  | var x =>
+    cases HT with | var HT =>
+    simp [Tm.up]
+    split
+    next H =>
+      constructor
+      simp_all [FinMap.lookup_left H]
+    next H =>
+      constructor
+      grind [FinMap.lookup_right]
+  | abs M IH =>
+    cases HT with | abs HT =>
+    rename_i T1 T2
+    simp [Tm.up]
+    constructor
+    conv =>
+      pattern T1 :: (Γ1 ++ (Γ3 ++ Γ2))
+      change (T1 :: Γ1) ++ (Γ3 ++ Γ2)
+    apply IH
+    simp_all
+    exact HT
+  | app M1 M2 IH1 IH2 =>
+    cases HT with | app H1 H2 =>
+    simp [Tm.up]
+    constructor
+    . apply IH1
+      exact H1
+    . apply IH2
+      exact H2
+
+
+def Typing.weaken_app {Γ1 Γ2: Context} {M: Tm} {T}:
+  Typing Γ1 M T ->
+  Typing (Γ2 ++ Γ1) (M.up 0 Γ2.length) T
+:= by
+  intro H
+  conv at H =>
+    arg 1
+    change [] ++ Γ1
+  conv =>
+    pattern (Γ2 ++ Γ1)
+    change [] ++ (Γ2 ++ Γ1)
+  apply weaken_lemma
+  exact H
+
+
+theorem Typing.bound {Γ: Context} {t T}:
+  Typing Γ t T -> t.bound ≤ Γ.length
+:= by
+  intro H
+  induction H with
+  | var H =>
+    simp [Tm.bound]
+    replace H := FinMap.lookup_some_lt H
+    omega
+  | app =>
+    simp [Tm.bound]
+    omega
+  | abs H IH =>
+    simp [Tm.bound] at *
+    exact IH
+
+
+def soundness_var {Δ Γ: Context} {i} {env: Env} {T}:
+  (H: Γ.lookup i = some T) ->
+  (S: Satisfy Δ env Γ) ->
+  forces Tm.NF Δ (env[i]'(by apply S.some_lt H)) T
+:= by
+  intro H S
+  match env with
+  | [] =>
+    cases S
+    contradiction
+  | x :: xs =>
+    match i with
+    | 0 =>
+      simp
+      match Γ with
+      | [] => contradiction
+      | T :: Ts =>
+        simp_all
+        cases S with | cons F _ =>
+        rewrite [<-H]
+        exact F
+    | i + 1 =>
+      simp_all
+      match Γ with
+      | [] => contradiction
+      | T :: Ts =>
+        simp at H
+        cases S with | cons F S =>
+        apply soundness_var H S
+
+
+def soundness {Γ: Context} {t T}:
+  Typing Γ t T ->
+  forall Δ env, Satisfy Δ env Γ -> forces Tm.NF Δ (t.msubst env) T
+:= by
+  intro HT Δ env S
+  induction t using Tm.ind generalizing Γ T Δ env with
+  | var x =>
+    cases HT with | var H =>
+    simp [Tm.msubst, Tm.msubst_var_lt (S.some_lt H)]
+    apply soundness_var H S
+  | app t1 t2 IH1 IH2 =>
+    cases HT with | app HT1 HT2 =>
+    rename_i A
+    specialize IH1 HT1 _ _ S
+    specialize IH2 HT2 _ _ S
+    simp [Tm.msubst]
+    simp [forces] at IH1
+    specialize IH1 (t2.msubst env) []
+    simp at IH1
+    apply IH1
+    exact IH2
+  | abs t IH =>
+    cases HT with | abs HT =>
+    rename_i T1 T2
+    specialize IH HT
+    simp [forces]
+    intro s Δ' F
+    obtain ⟨s', E, N⟩ := quote F
+    have K: Satisfy (Δ' ++ Δ) (s :: env.up 0 Δ'.length) (T1 :: Γ) := by
+      apply Satisfy.cons
+      . exact F
+      . apply Satisfy.weaken
+        exact S
+    specialize IH _ _ K
+    apply forces_eq
+    . apply ECl.symm
+      apply ECl.inclusion
+      apply Tm.step.compute
+      apply Tm.step.appAbs
+      apply Tm.msubst_le_step
+      replace HT := HT.bound
+      simp at HT
+      replace S := S.length
+      rewrite [S]
+      exact HT
+    . exact IH
+
+
+def normalize {Γ t T}:
+  Typing Γ t T ->
+  {t': Tm // t.eq t' ∧ Tm.NF Γ t' T}
+:= by
+  intro HT
+  let entailment := soundness HT
+  specialize entailment Γ (Env.vars Γ.length) (Satisfy.self)
+  simp at entailment
+  apply quote entailment
+
+
+namespace Example
+
+
+def var1: Typing Γ (.var 1) (.imp .Atom .Atom) := by
+  constructor
+  simp [Γ]
+
+
+scoped macro "typing": tactic => `(tactic| repeat (constructor <;> try (simp; eq_refl)))
+
+def varApp (n: Nat): Tm -> Tm := (Tm.var n).app
+
+
+def ChurchNum: Ty := (Ty.Atom.imp Ty.Atom).imp (Ty.Atom.imp Ty.Atom)
+
+
+def cn_2: Typing [] (.abs $ .abs $ varApp 1 $ varApp 1 $ (.var 0)) ChurchNum := by
+  typing
+
+
+def cn_3: Typing [] (.abs $ .abs $ varApp 1 $ varApp 1 $ varApp 1 $ (.var 0)) ChurchNum := by
+  typing
+
+
+/--
+λc₁.λc₂.(λs.λz. c₂ s (c₁ s z))
+ 3   2    1  0. (2  1) ((3  1) 0)
+-/
+def cn_add: Typing []
+  (.abs $ .abs $ .abs $ .abs $ (varApp 2 (.var 1)).app ((varApp 3 (.var 1)).app (.var 0)))
+  (ChurchNum.imp (ChurchNum.imp ChurchNum))
+:= by
+  typing
+
+
+-- try evaluate them
+-- #eval normalize cn_2
+-- #eval normalize ((cn_add.app cn_2).app cn_3)
+
+
+end Example
